

Linear algebra homework rework 2025/09/29

largeoyos

September 30, 2025

Problem.4

$$\begin{aligned}
 & \begin{vmatrix} x_1 & y & \cdots & y \\ z & x_2 & \cdots & y \\ \vdots & \vdots & \ddots & \vdots \\ z & z & \cdots & x_n \end{vmatrix} = \begin{vmatrix} x_1 & y & \cdots & y \\ z & x_2 & \cdots & y \\ \vdots & \vdots & \ddots & \vdots \\ z & z & \cdots & y + (x_n - y) \end{vmatrix} = (x_n - y) \cdot D_{n-1} + \\
 & \begin{vmatrix} x_1 & y & y & \cdots & y & y \\ z & x_2 & y & \cdots & y & y \\ z & z & x_3 & \cdots & y & y \\ \vdots & \vdots & \vdots & \ddots & \vdots & \vdots \\ z & z & z & \cdots & x_{n-1} & y \\ z & z & z & \cdots & z & y \end{vmatrix} \\
 & = (x_n - y) \cdot D_{n-1} + \begin{vmatrix} x_1 & y & y & \cdots & y & y \\ z - x_1 & x_2 - y & 0 & \cdots & 0 & 0 \\ z - x_1 & z - y & 0 & \cdots & 0 & 0 \\ \vdots & \vdots & \vdots & \ddots & \vdots & \vdots \\ z - x_1 & z - y & z - y & \cdots & x_{n-1} - y & 0 \\ z - x_1 & z - y & z - y & \cdots & z - y & 0 \end{vmatrix}_n \\
 & = (x_n - y) \cdot D_{n-1} + (-1)^{n+1} y \begin{vmatrix} z - x_1 & x_2 - y & 0 & \cdots & 0 \\ z - x_1 & z - y & x_3 - y & \cdots & 0 \\ \vdots & \vdots & \vdots & \ddots & \vdots \\ z - x_1 & z - y & z - y & \cdots & x_{n-1} - y \\ z - x_1 & z - y & z - y & \cdots & z - y \end{vmatrix}_{n-1} \\
 & = (x_n - y) \cdot D_{n-1} + (-1)^{n+1} y \begin{vmatrix} z - x_1 & x_2 - y & 0 & \cdots & 0 \\ 0 & z - x_2 & x_3 - y & \cdots & 0 \\ \vdots & \vdots & \vdots & \ddots & \vdots \\ 0 & 0 & 0 & \cdots & x_{n-1} - y \\ 0 & 0 & 0 & \cdots & z - x_{n-1} \end{vmatrix}_{n-1} \\
 & = (x_n - y) \cdot D_{n-1} + (-1)^{n+1} y \cdot \prod_{i=1}^{n-1} (z - x_i)
 \end{aligned}$$

Hence $D_n = (x_n - y) \cdot +y \cdot \prod_{i=1}^{n-1} (x_i - z)$
 Similarly, $D_n = (x_n - z) \cdot +y \cdot \prod_{i=1}^{n-1} (x_i - y)$

$$\text{when } y \neq z, D_n = \frac{y \prod_{i=1}^n (x_i - z) - x \prod_{i=1}^n (x_i - y)}{y - z}$$